\documentclass{article} % For LaTeX2e
% \usepackage{nips13submit_e,times}
\usepackage{xeCJK}
\setCJKmainfont{SimSun}
\usepackage{hyperref}
\usepackage{url}
\usepackage{graphicx}
\usepackage{amsmath}
\usepackage{amssymb}
\usepackage{algorithm}
\usepackage{algorithmic}
\usepackage{textcomp}  % \textcelsius
% \graphicspath{{./fig/}}
% \usepackage{tikz}

\title{Homework 3}
\author{Zhong Yun 2016K8009915009}
\date{Oct 8ï¼Œ2018}
\usepackage{geometry}
\geometry{left=2.5cm,right=2.5cm,top=2.5cm,bottom=2.5cm}



\newcommand{\fix}{\marginpar{FIX}}
\newcommand{\new}{\marginpar{NEW}}

\newtheorem{theorem}{Theorem}
\newtheorem{lemma}{Lemma}
\newtheorem{proof}{Proof}

\begin{document}


\maketitle
%
%\begin{abstract}
%empty
%\end{abstract}


% \input{problem-and-notation.tex}
%\input{aaa}

\section{Answer Sheet}
\begin{theorem}AdaBoost Algorithm

$$\frac{1}{N}\sum_{i=1}^NI(f(x_i)\neq y_i)\leq exp(-2\sum_{k=1}^K\gamma_k^2)$$

where $\gamma_k=\frac{1}{2}-\epsilon^{(k)}$

$$ I(f(x_i)\neq y_i)=\left\{
\begin{aligned}
0,while f(x_i)=y_i \\
1,while f(x_i)\neq y_i
\end{aligned}
\right.
$$
\end{theorem}

\begin{lemma}
$$\prod_{k=1}^K\sqrt{1-4\gamma_k^2}\leq e^{-2\sum_{k=1}^K\gamma_k^2}$$

where $\gamma_k\geq 0$
\end{lemma}
\begin{proof}
\begin{itemize}
\item[1.] \emph{We need to clarify some definitions:}
$$\alpha^{(k)}=\frac{1}{2}log(\frac{1-\epsilon^{(k)}}{\epsilon^{(k)}})$$
$$d_{i}^{(k+1)}=\frac{d_{i}^k}{Z^{(k)}}exp(-\alpha^{(k)}y_if(x_i))$$
$$\epsilon^{(k)}=\sum_{i=1}^Nd_i^{k-1}[y_i\neq f^{(k)}(x_i)]$$
$$Z^{(k)}=\sum_{i=1}^Nd_{i}^kexp(-\alpha^{(k)}y_if(x_i))$$
$$F(x)=\sum_{k=1}^K\alpha^{(k)}f^{(k)}(x)$$
$$f(x)=sgn[F(x)]=sgn[\sum_{k}\alpha^{(k)}f^{(k)}(x)]$$


\item[2.] \emph{According to Lemma, we only need to prove the following inequality:}
$$\frac{1}{N}\sum_{i=1}^NI(f(x_i)\neq y_i)\leq \prod_{k=1}^K\sqrt{1-4\gamma_k^2}$$

\item[3.] \emph{First, we prove this inequality}
$$\sum_{i=1}^NI(f(x_i)\neq y_i)\leq \sum_{i=1}^Nexp(-y_iF(x_i))$$

\emph{Proof:}

\emph{If} $f(x_i)=y_i$, \emph{then} $I(f(x_i)\neq y_i)=0$ \emph{and} $y_iF(x_i)\geq 0$, \emph{so} $exp(-y_iF(x_i))\geq 0$

\emph{We have} $I(f(x_i)\neq y_i)\leq exp(-y_iF(x_i))$

\emph{If} $f(x_i)\neq y_i$, \emph{then} $I(f(x_i)\neq y_i)=1$ \emph{and} $y_iF(x_i)\leq 0$, \emph{so} $exp(-y_iF(x_i))\geq 1$

\emph{Still, we have} $I(f(x_i)\neq y_i)\leq exp(-y_iF(x_i))$

\item[4.] \emph{We prove that:}
$$\frac{1}{N}\sum_{i=1}^Nexp(-y_iF(x_i))=\prod_{k=1}^KZ^{(k)}$$

\emph{Proof:\\According to the definition in part1, we have that}
$$\alpha^{(k)}=\frac{1}{2}log(\frac{1-\epsilon^{(k)}}{\epsilon^{(k)}})$$
$$d_{i}^{(k+1)}=\frac{d_{i}^k}{Z^{(k)}}exp(-\alpha^{(k)}y_if(x_i))$$
$$\epsilon^{(k)}=\sum_{i=1}^Nd_i^{k-1}[y_i\neq f^{(k)}(x_i)]$$
$$Z^{(k)}=\sum_{i=1}^Nd_{i}^kexp(-\alpha^{(k)}y_if(x_i))$$

$$
\begin{aligned}
\frac{1}{N}\sum_{i=1}^Nexp(-y_iF(x_i))&=\frac{1}{N}\sum_{i=1}^Nexp(-\sum_{k=1}^K\alpha^{(k)}y_if^{(k)}(x_i)\\
&=\sum_{i=1}^N\frac{1}{N}\prod_{k=1}^Kexp(\alpha^{(k)}y_if^{(k)}(x_i))\\
&=\sum_{i=1}^Nd_i^{(0)}\prod_{k=1}^Kexp(\alpha^{(k)}y_if^{(k)}(x_i))\\
&=Z^{(1)}\sum_{i=1}^Nd_i^{(1)}\prod_{k=2}^Kexp(\alpha^{(k)}y_if^{(k)}(x_i))\\
&=Z^{(1)}Z^{(2)}\sum_{i=1}^Nd_i^{(2)}\prod_{k=3}^Kexp(\alpha^{(k)}y_if^{(k)}(x_i))\\
&=\cdots\\
&=Z^{(1)}Z^{(2)}\cdots Z^{(K-1)}\sum_{i=1}^Nd_i^{(K)}exp(\alpha^{(K)}y_if^{(K)}(x_K))\\
&=Z^{(1)}Z^{(2)}\cdots Z^{(K)}\\
&=\prod_{k=1}^KZ^{(k)}
\end{aligned}
$$

\item[5.] \emph{We prove the following equality:}
$$Z^{(k)}=\sqrt{1-4\gamma_k^2}$$
\emph{where} $\gamma_k=\frac{1}{2}-\epsilon^{(k)}$

\emph{Proof:}
$$
\begin{aligned}
Z^{(k)}&=\sum_{i=1}^Nd_{i}^kexp(-\alpha^{(k)}y_if^{(k)}(x_i))\\
&=\sum_{f^{(k)}(x_i)=y_i}d_{i}^kexp(-\alpha^{(k)})+\sum_{f^{(k)}(x_i)\neq y_i}d_{i}^kexp(\alpha^{(k)})\\
&=(1-\epsilon^{(k)})exp(-\alpha^{(k)})+(\epsilon^{(k)})exp(\alpha^{(k)})\\
&=\sqrt{1-4\gamma_k^2}
\end{aligned}
$$
\emph{where} $\gamma_k=\frac{1}{2}-\epsilon^{(k)}$

\item[6.] \emph{Taking 1,\ 2,\ 3,\ 4,\ 5\ into acount,
We can prove that:}
$$\frac{1}{N}\sum_{i=1}^NI(f(x_i)\neq y_i)\leq exp(-2\sum_{k=1}^K\gamma_k^2)$$

\end{itemize}

\end{proof}





\end{document}
