\documentclass{article}
\usepackage{CJK}
\usepackage{amssymb} % For LaTeX2e
% \usepackage{nips13submit_e,times}
\usepackage{hyperref}
\usepackage{url}
\usepackage{graphicx}
\usepackage{amsmath}
\usepackage{algorithm}
\usepackage{algorithmic}
\usepackage{textcomp}  % \textcelsius
% \graphicspath{{./fig/}}
% \usepackage{tikz}

\title{Homework 1}
\author{Zhong Yun 2016K8009915009}
\usepackage{geometry}
\geometry{left=2.5cm,right=2.5cm,top=2.5cm,bottom=2.5cm}



\newcommand{\fix}{\marginpar{FIX}}
\newcommand{\new}{\marginpar{NEW}}
\newtheorem{theorem}{Theorem}
\newtheorem{proof}{Proof}


\begin{document}
\begin{CJK*}{GBK}{song}
\maketitle

\begin{theorem}
定理2.6.4
\begin{itemize}
  \item [(i)]  $A\rightarrow B, A \vdash B$
  \item [(ii)]  $A\rightarrow B, B\rightarrow C \vdash A\rightarrow C$
  \item [(iii)]  $A\rightarrow (B\rightarrow C), A\rightarrow B \vdash A\rightarrow C$
\end{itemize}
\end{theorem}


\begin{proof}证明如下：

\textbf{(i)}
\begin{tabbing}\hspace*{10bp}\=article\quad\quad\quad\quad\quad\quad\quad\quad\quad\quad\=$(\in)$\kill
\>$(1)A\rightarrow B,A\vdash A\rightarrow B$    \>$(\in)$\\
\>$(2)A\rightarrow B,A\vdash B$                 \>$(\in)$\\
\>$(3)A\rightarrow B, A \vdash B$               \>$((1)(2)(\rightarrow -))$ \qquad $\Box$\\
\end{tabbing}

\textbf{(ii)}
\begin{tabbing}\hspace*{10bp}\=article\quad\quad\quad\quad\quad\quad\quad\quad\quad\quad\=$(\in)$\kill
\>$(1)A,B\vdash A$    \>$(\in)$\\
\>$(2)A\vdash B\rightarrow A$      \>$((1)(\rightarrow +))$ \qquad $\Box$\\
\end{tabbing}

\textbf{(iii)}
\begin{tabbing}\hspace*{10bp}\=article\quad\quad\quad\quad\quad\quad\quad\quad\quad\quad\quad\quad\quad\quad\quad\quad\quad\quad\=$(\in)$\kill
\>$(1)A\rightarrow (B\rightarrow C),A\rightarrow B,A\vdash A$  \>$(\in)$\\
\>$(2)A\rightarrow (B\rightarrow C),A\rightarrow B,A\vdash A\rightarrow B$  \>$(\in)$\\
\>$(3)A\rightarrow (B\rightarrow C),A\rightarrow B,A\vdash B$  \>$((1)(2)(\rightarrow -))$\\
\>$(4)A\rightarrow (B\rightarrow C),A\rightarrow B,A\vdash A\rightarrow (B\rightarrow C)$  \>$(\in)$\\
\>$(5)A\rightarrow (B\rightarrow C),A\rightarrow B,A\vdash B\rightarrow C$  \>$((1)(4)(\rightarrow -))$\\
\>$(6)A\rightarrow (B\rightarrow C),A\rightarrow B,A\vdash C$  \>$((3)(5)(\rightarrow -))$\\
\>$(7)A\rightarrow (B\rightarrow C),A\rightarrow B\vdash A\rightarrow C$  \>$((6)(\rightarrow +))$ \qquad $\Box$\\
\end{tabbing}
\end{proof}

\begin{theorem}
定理2.6.9
\begin{itemize}
  \item [(i)]  $A\vdash B, A B.$
  \item [(ii)] $A\vee B \vdash \dashv B\vee A.(\vee 交换律)$
  \item [(iii)] $(A\vee B)\vee C \vdash \dashv A\vee (B\vee C).(\vee 结合律)$
  \item [(iv)] $A\vee B \vdash \dashv \neg A\rightarrow B$
  \item [(v )] $A\rightarrow B\vdash \dashv \neg A\vee B$
  \item [(vi)] $\neg(A\vee B)\vdash \dashv \neg A\wedge \neg B. (De Morgen律)$
  \item [(vii)] $\neg(A\wedge B)\vdash \dashv \neg A\vee \neg B. (De Morgen律)$
  \item [(viii)] $\O \vdash A\vee \neg A. (排中律)$
\end{itemize}
\end{theorem}


\begin{proof}证明如下：

\textbf{(i)}
\begin{tabbing}\hspace*{10bp}\=article\quad\quad\quad\quad\quad\quad\quad\quad\quad\quad\=$(\in)$\kill
\>$(1)A\vdash A$  \>$(\in)$\\
\>$(2)A\vdash A\vee B,\quad A\vdash B\vee A$  \>$((1)(\vee+))$\\
\>$(3)A\vdash A\vee B,B\vee A$  \>$(2)$ \qquad $\Box$\\
\end{tabbing}

\textbf{(ii)}

先证$A\vee B\vdash B\vee A$
\begin{tabbing}\hspace*{10bp}\=article\quad\quad\quad\quad\quad\quad\quad\quad\quad\quad\quad\quad\quad\quad\quad\quad\quad\quad\quad\quad\= 由定理2.6.9(i)\kill
\>$(1)A\vdash B\vee A,\quad B\vdash B\vee A$  \>(由定理$2.6.9(i)$)\\
\>$(2)A\vee B,A\vdash B\vee A,\quad A\vee B,B\vdash B\vee A$  \>$((1)(\vee+))$\\
\>$(3)A\vee B,A\vee B\vdash B\vee A$，即$A\vee B\vdash B\vee A$  \>$((2)(\vee-))$\\
\end{tabbing}

再证$B\vee A\vdash A\vee B$
\begin{tabbing}\hspace*{10bp}\=article\quad\quad\quad\quad\quad\quad\quad\quad\quad\quad\quad\quad\quad\quad\quad\quad\quad\quad\quad\quad\= 由定理2.6.9(i)\kill
\>$(1)B\vdash A\vee B,\quad A\vdash A\vee B$  \>(由定理$2.6.9(i)$)\\
\>$(2)B\vee A,B\vdash A\vee B,\quad B\vee A,A\vdash A\vee B$  \>$((1)(\vee+))$\\
\>$(3)B\vee A,B\vee A\vdash A\vee B$，即$B\vee A\vdash A\vee B$  \>$((2)(\vee-))$\\
\end{tabbing}

综上$$A\vee B\vdash\dashv B\vee A \qquad \Box$$

\textbf{(iii)}

先证$(A\vee B)\vee C\vdash A\vee(B\vee C)$
\begin{tabbing}\hspace*{10bp}\=article\quad\quad\quad\quad\quad\quad\quad\quad\quad\quad\quad\quad\quad\quad\quad\quad\quad\quad\quad\quad\= 由定理2.6.9(i)\kill
\>$(1)A\vdash A\vee(B\vee C)$  \>(由定理$2.6.9(i)$)\\
\>$(2)B\vdash B\vee C$  \>(由定理$2.6.9(i)$)\\
\>$(3)B\vdash A\vee(B\vee C)$  \>$((2)(\vee+))$\\
\>$(4)A\vee B\vdash A\vee(B\vee C)$  \>$((1)(3)(\vee-))$\\
\>$(5)C\vdash B\vee C$  \>(由定理$2.6.9(i)$)\\
\>$(6)C\vdash A\vee(B\vee C)$  \>$((5)(\vee+))$\\
\>$(7)(A\vee B)\vee C\vdash A\vee(B\vee C)$  \>$((4)(6)(\vee-))$\\
\end{tabbing}

再证$A\vee(B\vee C)\vdash (A\vee B)\vee C$
\begin{tabbing}\hspace*{10bp}\=article\quad\quad\quad\quad\quad\quad\quad\quad\quad\quad\quad\quad\quad\quad\quad\quad\quad\quad\quad\quad\= 由定理2.6.9(i)\kill
\>$(1)C\vdash (A\vee B)\vee C$  \>(由定理$2.6.9(i)$)\\
\>$(2)B\vdash A\vee B$  \>(由定理$2.6.9(i)$)\\
\>$(3)B\vdash (A\vee B)\vee C$  \>$((2)(\vee+))$\\
\>$(4)B\vee C\vdash (A\vee B)\vee C$  \>$((1)(3)(\vee-))$\\
\>$(5)A\vdash A\vee B$  \>(由定理$2.6.9(i)$)\\
\>$(6)A\vdash (A\vee B)\vee C$  \>$((5)(\vee+))$\\
\>$(7)A\vee(B\vee C)\vdash (A\vee B)\vee C$  \>$((4)(6)(\vee-))$\\
\end{tabbing}

综上$$(A\vee B)\vee C\vdash\dashv A\vee(B\vee C) \qquad \Box$$

\textbf{(iv)}

先证$A\vee B \vdash \neg A\rightarrow B$
\begin{tabbing}\hspace*{10bp}\=article\quad\quad\quad\quad\quad\quad\quad\quad\quad\quad\quad\quad\quad\quad\quad\quad\quad\quad\quad\quad\= 由定理2.6.9(i)\kill
\>$(1)A\vdash \neg A\rightarrow B$  \>(由定理$2.6.5(v)$)\\
\>$(2)B\vdash \neg A\rightarrow B$  \>(由定理$2.6.4(ii)$)\\
\>$(3)A\vee B\vdash \neg A\rightarrow B$  \>$((1)(2)(\vee-))$\\
\end{tabbing}

再证$\neg A\rightarrow B \vdash A\vee B$
\begin{tabbing}\hspace*{10bp}\=article\quad\quad\quad\quad\quad\quad\quad\quad\quad\quad\quad\quad\quad\quad\quad\quad\quad\quad\quad\quad\= 由定理2.6.9(i)\kill
\>$(1)A\vdash A\vee B$  \>(由本定理$(i)$)\\
\>$(2)\neg (A\vee B)\vdash \neg A$  \>(由定理$2.6.6(v),(1)$)\\
\>$(3)\neg A\rightarrow B,\neg(A\vee B)\vdash \neg A$  \>$((2)(+))$\\
\>$(4)\neg A\rightarrow B,\neg(A\vee B)\vdash \neg A\rightarrow B$  \>($\in$)\\
\>$(5)\neg A\rightarrow B,\neg(A\vee B)\vdash B$  \>($(4),(3),(\rightarrow -)$)\\
\>$(6)\neg A\rightarrow B,\neg(A\vee B)\vdash A\vee B$  \>($(5),(\vee+)$)\\
\>$(7)\neg A\rightarrow B,\neg(A\vee B)\vdash \neg (A\vee B)$  \>($\in$)\\
\>$(8)\neg A\rightarrow B\vdash A\vee B$  \>($(6),(7),(\neg -)$)\qquad $\Box$
\end{tabbing}


\textbf{(v)}

先证$A\rightarrow B \vdash \neg A\vee B$
\begin{tabbing}\hspace*{10bp}\=article\quad\quad\quad\quad\quad\quad\quad\quad\quad\quad\quad\quad\quad\quad\quad\quad\quad\quad\quad\quad\= 由定理2.6.9(i)\kill
\>$(1)\neg A\vdash \neg A\vee B$  \>(由本定理$(i)$)\\
\>$(2)\neg (\neg A\vee B)\vdash A$  \>(由定理$2.6.6(v),(1)$)\\
\>$(3)A\rightarrow B,\neg(\neg A\vee B)\vdash A$  \>$((2)(+))$\\
\>$(4)A\rightarrow B,\neg(\neg A\vee B)\vdash A\rightarrow B$  \>($\in$)\\
\>$(5)A\rightarrow B,\neg(\neg A\vee B)\vdash B$  \>($(4),(3),(\rightarrow -)$)\\
\>$(6)A\rightarrow B,\neg(\neg A\vee B)\vdash \neg A\vee B$  \>($(5),(\vee+)$)\\
\>$(7)A\rightarrow B,\neg(\neg A\vee B)\vdash \neg (\neg A\vee B)$  \>($\in$)\\
\>$(8)A\rightarrow B\vdash \neg A\vee B$  \>($(6),(7),(\neg -)$)
\end{tabbing}

再证$\neg A\vee B \vdash A\rightarrow B$
\begin{tabbing}\hspace*{10bp}\=article\quad\quad\quad\quad\quad\quad\quad\quad\quad\quad\quad\quad\quad\quad\quad\quad\quad\quad\quad\quad\= 由定理2.6.9(i)\kill
\>$(1)\neg A\vdash A\rightarrow B$  \>(由定理$2.6.5(v)$)\\
\>$(2)B\vdash A\rightarrow B$  \>(由定理$2.6.4(ii)$)\\
\>$(3)\neg A\vee B\vdash A\rightarrow B$  \>$((1)(2)(\vee-))$ \qquad $\Box$
\end{tabbing}

\textbf{(vi)}

先证$\neg(A\vee B)\vdash \neg A\wedge \neg B$
\begin{tabbing}\hspace*{10bp}\=article\quad\quad\quad\quad\quad\quad\quad\quad\quad\quad\quad\quad\quad\quad\quad\quad\quad\quad\quad\quad\= 由定理2.6.9(i)\kill
\>$(1)\neg A\rightarrow B\vdash A\vee B$  \>(由本定理$(iv)$)\\
\>$(2)\neg (A\vee B)\vdash \neg(\neg A\rightarrow B)$  \>(由定理$2.6.6(v)$)\\
\>$(3)\neg (A\vee B),A\vdash \neg(\neg A\rightarrow B)$  \>$((\in ))$\\
\>$(4)A\vdash \neg A\rightarrow B$  \>(由定理$2.6.5(v)$)\\
\>$(5)\neg (A\vee B),A\vdash \neg A\rightarrow B$  \>$((\in))$\\
\>$(6)\neg (A\vee B)\vdash \neg A$  \>($(3),(5),(\neg -)$)\\
\>$(7)\neg B\rightarrow A\vdash B\vee A$  \>(由定理$2.6.9(iv)$)\\
\>$(8)\neg (A\vee B)\vdash \neg (\neg B\rightarrow A)$  \>(由定理$2.6.6(v)$)\\
\>$(9)\neg (A\vee B),B\vdash \neg (\neg B\rightarrow A)$  \>$((\in))$\\
\>$(10)B \vdash \neg B\rightarrow A$ \>(由定理$2.6.5(v)$)\\
\>$(11)\neg (A\vee B),B\vdash \neg B\rightarrow A$  \>$((\in))$\\
\>$(12)\neg (A\vee B),B\vdash \neg B$  \>($(9),(11),(\neg -)$)\\
\>$(13)\neg (A\vee B),B\vdash \neg A \wedge \neg B$  \>($(6),(12),(\wedge +)$)
\end{tabbing}

再证$\neg(A\vee B)\dashv \neg A\wedge \neg B$
\begin{tabbing}\hspace*{10bp}\=article\quad\quad\quad\quad\quad\quad\quad\quad\quad\quad\quad\quad\quad\quad\quad\quad\quad\quad\quad\quad\= 由定理2.6.9(i)\kill
\>$(1)\neg A\rightarrow B\vdash \neg (\neg A\wedge \neg B)$  \>(由定理$2.6.8(v)$)\\
\>$(2)\neg A\wedge \neg B\vdash \neg (\neg A\rightarrow B)$  \>(由定理$2.6.6(ii)$)\\
\>$(3)\neg A\wedge \neg B,A\vee B\vdash \neg (\neg A\rightarrow B)$  \>(($\in$))\\
\>$(4)A \vdash \neg A \rightarrow B$  \>(由定理$2.6.5(v)$)\\
\>$(5)B \vdash \neg A \rightarrow B$  \>(由定理$2.6.4(ii)$)\\
\>$(6)A\vee B\vdash \neg A \rightarrow B$ \>($(4),(5),(\vee -)$)\\
\>$(7)\neg A\wedge \neg B,A\vee B\vdash \neg A\rightarrow B$ \>(($\in$))\\
\>$(8)\neg A\wedge \neg B\vdash \neg(A\vee B)$ \>($(3),(7),(\neg -)$)\qquad$\Box$
\end{tabbing}

\textbf{(vii)}

先证$\neg(A\wedge B)\vdash \neg A\vee \neg B$
\begin{tabbing}\hspace*{10bp}\=article\quad\quad\quad\quad\quad\quad\quad\quad\quad\quad\quad\quad\quad\quad\quad\quad\quad\quad\quad\quad\= 由定理2.6.9(i)\kill
\>$(1)A\rightarrow \neg B\vdash \neg A\vee \neg B$  \>(由本定理$(iv)$)\\
\>$(2)\neg (\neg A\vee \neg B)\vdash \neg(A\rightarrow \neg B)$  \>(由定理$2.6.6(v)$)\\
\>$(3)\neg (\neg A\vee \neg B),\neg A\vdash \neg(A\rightarrow \neg B)$  \>$((\in ))$\\
\>$(4)\neg A\vdash A\rightarrow \neg B$  \>(由定理$2.6.5(v)$)\\
\>$(5)\neg (\neg A\vee \neg B),\neg A\vdash A\rightarrow \neg B$  \>$((\in))$\\
\>$(6)\neg (\neg A\vee \neg B)\vdash A$  \>($(3),(5),(\neg -)$)\\
\>$(7)B\rightarrow \neg A\vdash \neg B\vee \neg A$  \>(由定理$2.6.9(iv)$)\\
\>$(8)\neg (\neg A\vee \neg B)\vdash \neg (B\rightarrow \neg A)$  \>(由定理$2.6.6(v)$)\\
\>$(9)\neg (\neg A\vee \neg B),\neg B\vdash \neg (B\rightarrow \neg A)$  \>$((\in))$\\
\>$(10)\neg B \vdash B\rightarrow \neg A$ \>(由定理$2.6.5(v)$)\\
\>$(11)\neg (\neg A\vee \neg B),\neg B\vdash B\rightarrow A$  \>$((\in))$\\
\>$(12)\neg (\neg A\vee \neg B)\vdash B$  \>($(9),(11),(\neg -)$)\\
\>$(13)\neg (\neg A\vee \neg B)\vdash A \wedge B$  \>($(6),(12),(\wedge +)$)\\
\>$(14)\neg (A \wedge B)\vdash \neg A\vee \neg B$  \>(由定理$2.6.6(vii),(13)$)
\end{tabbing}

再证$\neg(A\wedge B)\dashv \neg A\vee \neg B$
\begin{tabbing}\hspace*{10bp}\=article\quad\quad\quad\quad\quad\quad\quad\quad\quad\quad\quad\quad\quad\quad\quad\quad\quad\quad\quad\quad\= 由定理2.6.9(i)\kill
\>$(1)A\rightarrow \neg B\vdash \neg (A\wedge B)$  \>(由定理$2.6.8(v)$)\\
\>$(2)A\wedge B\vdash \neg (A\rightarrow \neg B)$  \>(由定理$2.6.6(ii)$)\\
\>$(3)A\wedge B,\neg A\vee \neg B\vdash \neg (A\rightarrow \neg B)$  \>$((\in))$\\
\>$(4)\neg A \vdash A \rightarrow \neg B$  \>(由定理$2.6.5(v)$)\\
\>$(5)\neg B \vdash A \rightarrow \neg B$  \>(由定理$2.6.4(ii)$)\\
\>$(6)\neg A\vee \neg B\vdash A \rightarrow \neg B$ \>($(4),(5),(\vee -)$)\\
\>$(7)A\wedge B,\neg A\vee \neg B\vdash A\rightarrow \neg B$ \>$((\in))$\\
\>$(8)A\wedge B\vdash \neg(\neg A\vee \neg B)$ ($(3),(7),(\neg -)$)\\
\>$(9)\neg A\vee \neg B\vdash \neg(A\wedge B)$  \>(由定理$2.6.6(vi),(8)$)\qquad$\Box$
\end{tabbing}


\textbf{(viii)}

\begin{tabbing}\hspace*{10bp}\=article\quad\quad\quad\quad\quad\quad\quad\quad\quad\quad\quad\quad\quad\quad\quad\quad\quad\quad\quad\quad\= 由定理2.6.9(i)\kill
\>$(1)\O \vdash \neg (A \wedge \neg A)$  \>(由定理$2.6.8(vii)$)\\
\>$(2)\neg(\neg A\vee A)\vdash A \wedge \neg A$  \>(由定理$2.6.9(vi)$)\\
\>$(3)\O , \neg(\neg A\vee A)\vdash A \wedge \neg A$  \>$(\in )$\\
\>$(4)\O \vdash \neg A \vee A$  \>($(1)(3)(\neg -)$)\\
\>$(5)\O \vdash A \vee \neg A$  \>($\vee$ 交换律)\qquad$\Box$\\
\end{tabbing}


\end{proof}


\end{CJK*}
\end{document}


